AP/Util/Array.lean
@@ -1,0 +1,74 @@
+import AP.Util.List
+
+namespace Array
+
+variable {α β : Type*} {xs ys : Array α}
+
+def foldlWith' (xs : Array α) (f : β → (x : α) → x ∈ xs → β) (z : β) (i : ℕ) : β :=
+  if h : i < xs.size then xs.foldlWith' f (f z (xs[i]) (by simp)) (i + 1) else z
+
+def foldlWith (xs : Array α) (f : β → (x : α) → x ∈ xs → β) (z : β) : β :=
+  xs.foldlWith' f z 0
+
+theorem foldlWith'_cons' {xs : List α} {x : α}
+{f : β → (y : α) → y ∈ (⟨x :: xs⟩ : Array α) → β} {z : β} {i} (h : i ≠ 0) :
+(⟨x :: xs⟩ : Array α).foldlWith' f z i = (⟨xs⟩ : Array α).foldlWith'
+(λ acc x h₁ => f acc x # by simp at h₁; simp [h₁]) z (i - 1) := by
+  fun_induction foldlWith'
+  · nm r i h₁ ih
+    simp at ih ⊢
+    rw [ih]
+    clear ih
+    cases i; simp at h; nm i; clear h
+    nth_rw 2 [foldlWith']
+    split_ifs with h₂; simp
+    simp at h₁ h₂
+    linarith
+  · nm r i h₁
+    cases i; simp at h; nm i; clear h
+    simp at h₁ ⊢
+    unfold foldlWith'
+    simp
+    intro h₂
+    linarith
+
+@[simp]
+theorem foldlWith'_cons {xs : List α} {x : α}
+{f : β → (y : α) → y ∈ (⟨x :: xs⟩ : Array α) → β} {z : β} {i} :
+(⟨x :: xs⟩ : Array α).foldlWith' f z (i + 1) = (⟨xs⟩ : Array α).foldlWith'
+(λ acc x h₁ => f acc x # by simp at h₁; simp [h₁]) z i :=
+  foldlWith'_cons' # by simp
+
+theorem foldlWith_eq_foldlWith_toList {f : β → (x : α) → x ∈ xs → β} {z : β} :
+xs.foldlWith f z = xs.toList.foldlWith (λ acc x h => f acc x # by simp at h; exact h) z := by
+  classical
+  unfold foldlWith
+  rcases xs with ⟨xs⟩; dsimp
+  induction xs generalizing z
+  · unfold foldlWith'; simp
+  nm x xs ih
+  nth_rw 1 [foldlWith']
+  simp [ih]
+
+@[simp]
+theorem foldlWith_snoc {x : α} {f : β → (y : α) → y ∈ xs ++ [x] → β} {z : β} :
+(xs ++ [x]).foldlWith f z = f (xs.foldlWith (λ acc y h => f acc y (by simp [h])) z)
+x (by simp) := by
+  classical
+  rcases xs with ⟨xs⟩
+  simp [foldlWith_eq_foldlWith_toList, List.foldlWith_eq_foldl]
+  congr 1
+  apply List.foldl_eq_foldl_of_fn_congr
+  intro acc y hy
+  simp [hy]
+
+theorem foldlWith_eq_foldl [ha : DecidableEq α] {f : β → (x : α) → x ∈ xs → β} {z : β} :
+xs.foldlWith f z = xs.foldl (λ acc x => if h : x ∈ xs then f acc x h else z) z := by
+  rcases xs with ⟨xs⟩
+  rw [foldlWith_eq_foldlWith_toList, ←foldl_toList, List.foldlWith_eq_foldl]
+  apply List.foldl_eq_foldl_of_fn_congr
+  intro acc x hx; simp [hx]
+
+theorem foldlWith_eq_foldl_toList [ha : DecidableEq α] {f : β → (x : α) → x ∈ xs → β} {z : β} :
+xs.foldlWith f z = xs.toList.foldl (λ acc x => if h : x ∈ xs then f acc x h else z) z := by
+  simp; exact foldlWith_eq_foldl
